Added cem and expr_db_nat, working natural semantics

expr_db.v
@@ -1,7 +1,8 @@
 Require Vector.
 
+Definition db_ind := Fin.t.
 Inductive expr (n : nat) : Type := 
-  | var : Fin.t n -> expr n
+  | var : db_ind n -> expr n
   | lam : expr (S n) -> expr n
   | app : expr n -> expr n -> expr n.
 
@@ -12,7 +13,7 @@ Definition value {n} (t : expr n) : Prop := match t with
 
 Notation " :λ N " := (forall n, lam n N) (at level 20).
 Notation " M @ N " := (forall n, app n M N) (at level 60). 
-Coercion var : Fin.t >-> expr.
+Coercion var : db_ind >-> expr.
 
 Example term_1 : expr 0 := lam 0 (var 1 Fin.F1).
 Example term_2 : expr 0 := app 0 term_1 term_1.
