cem.v
@@ -1,0 +1,38 @@
+Require Import expr_db_nat.
+Require Import Unicode.Utf8_core.
+
+Definition append := Datatypes.app.
+
+Inductive closure : Type := 
+  | close : expr -> nat -> closure. 
+
+Inductive cell : Type :=
+  | cl : closure -> nat -> cell.
+
+Definition heap := list (prod nat cell).
+
+Inductive configuration : Type :=
+  | st : heap -> closure -> configuration.
+
+Notation " x ↦ M " := (x, M) (at level 40).
+Notation " ⟨ Φ ⟩ m " := (st Φ m) (at level 40).
+Notation " ⟨ Ψ , b ⟩ N " := (st (cons b Ψ) N) (at level 40).
+Notation " ⟨ Φ , b , Ψ ⟩ N " := (st (append _ Ψ (cons b Φ)) N) (at level 40).
+Notation " { M , e } " := (cl M e).
+Notation " < M , e > " := (close M e).
+
+Inductive cactus_lookup : nat -> nat -> heap -> nat -> Prop :=
+  | zero : forall x Φ M Υ, cactus_lookup 0 x (append _ Φ (cons (x ↦ M) Υ)) x
+  | pred : forall x y z Φ M Υ i, cactus_lookup i x Φ z -> 
+            cactus_lookup (S i) y (append _ Φ (cons (y ↦ {M, x}) Υ)) z.
+
+Reserved Notation " c1 '⇓' c2 " (at level 50).
+Inductive step : configuration -> configuration -> Prop :=
+  | Id : ∀ M V x y z Φ Ψ Υ v, cactus_lookup v z Φ x -> ⟨Φ⟩M ⇓ ⟨Ψ⟩V ->
+      ⟨Φ, x ↦ {M, y}, Υ⟩close (var v) z ⇓ ⟨Ψ, x ↦ {V, y}, Υ⟩V
+  | Abs : ∀ N Φ e, ⟨Φ⟩close (:λN) e ⇓ ⟨Φ⟩close (:λN) e
+  | App : ∀ N M Φ Ψ Υ V f e ne, ⟨Φ⟩close M e ⇓ ⟨Ψ⟩close (:λN) ne ->
+      ⟨Ψ, f ↦ {close M e, ne}⟩close N f ⇓ ⟨Υ⟩V -> 
+              ⟨Φ⟩close (M@N) e ⇓ ⟨Υ⟩V
+where " c1 '⇓' c2 " := (step c1 c2).
+
