expr_db_nat.v
@@ -1,0 +1,18 @@
+Inductive expr : Type := 
+  | var : nat -> expr 
+  | lam : expr -> expr
+  | app : expr -> expr -> expr.
+
+Definition value (t : expr) : Prop := match t with
+  | lam _ => True
+  | _ => False
+  end.
+
+Notation " :λ N " := (lam N) (at level 20).
+Notation " M @ N " := (app M N) (at level 60). 
+Coercion var : nat >-> expr.
+
+Example term_1 : expr := lam (var 0).
+Example term_2 : expr := app term_1 term_1.
+
+
